@@ -1,0 +1,10 @@
+/-
+`sys_sbrk` meets its specification, given `argint`, `myproc` and `growproc`.
+-/
+import Xv6.ProofSysSbrk
+
+namespace Xv6
+
+theorem SysSbrk (AI : ARGINT) (MP : MYPROC) (GP : GROWPROC) : SYSSBRK := sys_sbrk_proof AI MP GP
+
+end Xv6
